lib/DataStructures/BtreeModel.i.dfy
@@ -132,6 +132,161 @@ abstract module BtreeModel {
     }
   }
 
+  lemma IndexesNonempty(node: Node)
+    requires WF(node)
+    requires node.Index?
+    ensures 0 < |Interpretation(node)|
+  {
+    var child := node.children[0];
+    if child.Leaf? {
+      reveal_Interpretation();
+      reveal_AllKeys();
+      assert 0 < |child.keys|;
+      var key := child.keys[0];
+      assert key  in Interpretation(child);
+      assert key in AllKeys(child);
+      if 0 < |node.pivots| {
+        assert AllKeysBelowBound(node, 0);
+        assert Keys.LargestLte(node.pivots, key) == -1;
+      } else {
+        assert Keys.LargestLte(node.pivots, key) == -1;
+      }
+      InterpretationDelegation(node, key);
+    } else {
+      IndexesNonempty(child);
+      var key :| key in Interpretation(child);
+      AllKeysIsConsistentWithInterpretation(child, key);
+      assert key in AllKeys(child);
+      if 0 < |node.pivots| {
+        assert AllKeysBelowBound(node, 0);
+        assert Keys.LargestLte(node.pivots, key) == -1;
+      } else {
+        assert Keys.LargestLte(node.pivots, key) == -1;
+      }
+      InterpretationDelegation(node, key);      
+    }
+  }
+  
+  lemma ChildOfIndexNonempty(node: Node, i: nat)
+    requires WF(node)
+    requires node.Index?
+    requires i < |node.children|
+    ensures 0 < |Interpretation(node.children[i])|
+  {
+    var child := node.children[i];
+    if child.Leaf? {
+      reveal_Interpretation();
+      reveal_AllKeys();
+      assert 0 < |child.keys|;
+      var key := child.keys[0];
+      assert key  in Interpretation(child);      
+    } else {
+      IndexesNonempty(child);
+    }
+  }
+  
+  function MinKey(node: Node) : (result: Key)
+    requires WF(node)
+    requires 0 < |Interpretation(node)|
+  {
+    if node.Leaf? then (
+      assert |node.keys| == 0 ==> Interpretation(node) == map[] by {
+        reveal_Interpretation();
+      }
+      node.keys[0]
+    ) else (
+      ChildOfIndexNonempty(node, 0);
+      MinKey(node.children[0])
+    )
+  }
+
+  lemma MinKeyProperties(node: Node)
+    requires WF(node)
+    requires 0 < |Interpretation(node)|
+    ensures MinKey(node) in Interpretation(node)
+    ensures forall key | key in Interpretation(node) :: Keys.lte(MinKey(node), key)
+  {
+    var result := MinKey(node);
+    if node.Leaf? {
+      reveal_Interpretation();
+    } else {
+      var child := node.children[0];
+      ChildOfIndexNonempty(node, 0);
+      MinKeyProperties(child);
+      if 0 < |node.pivots| {
+        assert AllKeysBelowBound(node, 0);
+        AllKeysIsConsistentWithInterpretation(child, result);
+        assert Keys.LargestLte(node.pivots, result) == -1;
+      } else {
+        assert Keys.LargestLte(node.pivots, result) == -1;
+      }
+      InterpretationDelegation(node, result);
+      forall key | key in Interpretation(node)
+        ensures Keys.lte(result, key)
+      {
+        var keyidx := 1 + Keys.LargestLte(node.pivots, key);
+        InterpretationInheritance(node, key);
+        if keyidx == 0 {
+        } else {
+          assert AllKeysBelowBound(node, 0);
+          Keys.IsStrictlySortedImpliesLte(node.pivots, 0, keyidx-1);
+          assert AllKeysAboveBound(node, keyidx);
+        }
+      }
+    }
+  }
+
+  function MaxKey(node: Node) : (result: Key)
+    requires WF(node)
+    requires 0 < |Interpretation(node)|
+  {
+    if node.Leaf? then (
+      assert |node.keys| == 0 ==> Interpretation(node) == map[] by {
+        reveal_Interpretation();
+      }
+      Last(node.keys)
+    ) else (
+      ChildOfIndexNonempty(node, |node.children| - 1);
+      MaxKey(Last(node.children))
+    )
+  }
+
+  lemma MaxKeyProperties(node: Node)
+    requires WF(node)
+    requires 0 < |Interpretation(node)|
+    ensures MaxKey(node) in Interpretation(node)
+    ensures forall key | key in Interpretation(node) :: Keys.lte(key, MaxKey(node))
+  {
+    var result := MaxKey(node);
+    if node.Leaf? {
+      reveal_Interpretation();
+    } else {
+      var child := Last(node.children);
+      ChildOfIndexNonempty(node, |node.children|-1);
+      MaxKeyProperties(child);
+      if 0 < |node.pivots| {
+        assert AllKeysAboveBound(node, |node.children|-1);
+        AllKeysIsConsistentWithInterpretation(child, result);
+        assert Keys.LargestLte(node.pivots, result) == |node.pivots|-1;
+      } else {
+        assert Keys.LargestLte(node.pivots, result) == |node.pivots|-1;
+      }
+      InterpretationDelegation(node, result);
+      forall key | key in Interpretation(node)
+        ensures Keys.lte(key, result)
+      {
+        var keyidx := 1 + Keys.LargestLte(node.pivots, key);
+        InterpretationInheritance(node, key);
+        if keyidx == |node.children| - 1 {
+        } else {
+          assert AllKeysBelowBound(node, keyidx);
+          Keys.IsStrictlySortedImpliesLte(node.pivots, keyidx, |node.pivots| - 1);
+          assert AllKeysAboveBound(node, |node.children| - 1);
+        }
+      }
+    }
+  }
+  
   predicate SplitLeaf(oldleaf: Node, leftleaf: Node, rightleaf: Node, pivot: Key)
   {
     && oldleaf.Leaf?
